examples/Employee_DesignModel_UMLPart.thy
@@ -1045,26 +1045,6 @@ lemma \<sigma>_modifiedonly: "(\<sigma>\<^sub>1,\<sigma>\<^sub>1') \<Turnstile> 
                  X\<^sub>P\<^sub>e\<^sub>r\<^sub>s\<^sub>o\<^sub>n1_def X\<^sub>P\<^sub>e\<^sub>r\<^sub>s\<^sub>o\<^sub>n2_def X\<^sub>P\<^sub>e\<^sub>r\<^sub>s\<^sub>o\<^sub>n3_def X\<^sub>P\<^sub>e\<^sub>r\<^sub>s\<^sub>o\<^sub>n4_def X\<^sub>P\<^sub>e\<^sub>r\<^sub>s\<^sub>o\<^sub>n5_def X\<^sub>P\<^sub>e\<^sub>r\<^sub>s\<^sub>o\<^sub>n6_def X\<^sub>P\<^sub>e\<^sub>r\<^sub>s\<^sub>o\<^sub>n7_def X\<^sub>P\<^sub>e\<^sub>r\<^sub>s\<^sub>o\<^sub>n8_def X\<^sub>P\<^sub>e\<^sub>r\<^sub>s\<^sub>o\<^sub>n9_def
                  person1_def person2_def person3_def person4_def person5_def person6_def person7_def person8_def person9_def
                  image_def)
- apply(simp add: including_rep_set mtSet_rep_set)
- apply(simp add: oid_of_option_def oid_of_type\<^sub>O\<^sub>c\<^sub>l\<^sub>A\<^sub>n\<^sub>y_def, clarsimp)
- apply(simp add: \<sigma>\<^sub>1_def \<sigma>\<^sub>1'_def
-                 oid0_def oid1_def oid2_def oid3_def oid4_def oid5_def oid6_def oid7_def oid8_def)
-done
-
-lemma \<sigma>_modifiedonly2: "(\<sigma>\<^sub>1,\<sigma>\<^sub>1') \<Turnstile> (Set{ X\<^sub>P\<^sub>e\<^sub>r\<^sub>s\<^sub>o\<^sub>n1 .oclAsType(OclAny)
-                      , X\<^sub>P\<^sub>e\<^sub>r\<^sub>s\<^sub>o\<^sub>n2 .oclAsType(OclAny)
-                    (*, X\<^sub>P\<^sub>e\<^sub>r\<^sub>s\<^sub>o\<^sub>n3 .oclAsType(OclAny)*)
-                      , X\<^sub>P\<^sub>e\<^sub>r\<^sub>s\<^sub>o\<^sub>n4 .oclAsType(OclAny)
-                    (*, X\<^sub>P\<^sub>e\<^sub>r\<^sub>s\<^sub>o\<^sub>n5 .oclAsType(OclAny)*)
-                      , X\<^sub>P\<^sub>e\<^sub>r\<^sub>s\<^sub>o\<^sub>n6 .oclAsType(OclAny)
-                    (*, X\<^sub>P\<^sub>e\<^sub>r\<^sub>s\<^sub>o\<^sub>n7 .oclAsType(OclAny)*)
-                    (*, X\<^sub>P\<^sub>e\<^sub>r\<^sub>s\<^sub>o\<^sub>n8 .oclAsType(OclAny)*)
-                    (*, X\<^sub>P\<^sub>e\<^sub>r\<^sub>s\<^sub>o\<^sub>n9 .oclAsType(OclAny)*)}->oclIsModifiedOnly2())"
- apply(simp add: OclIsModifiedOnly2_def OclValid_def
-                 oid0_def oid1_def oid2_def oid3_def oid4_def oid5_def oid6_def oid7_def oid8_def
-                 X\<^sub>P\<^sub>e\<^sub>r\<^sub>s\<^sub>o\<^sub>n1_def X\<^sub>P\<^sub>e\<^sub>r\<^sub>s\<^sub>o\<^sub>n2_def X\<^sub>P\<^sub>e\<^sub>r\<^sub>s\<^sub>o\<^sub>n3_def X\<^sub>P\<^sub>e\<^sub>r\<^sub>s\<^sub>o\<^sub>n4_def X\<^sub>P\<^sub>e\<^sub>r\<^sub>s\<^sub>o\<^sub>n5_def X\<^sub>P\<^sub>e\<^sub>r\<^sub>s\<^sub>o\<^sub>n6_def X\<^sub>P\<^sub>e\<^sub>r\<^sub>s\<^sub>o\<^sub>n7_def X\<^sub>P\<^sub>e\<^sub>r\<^sub>s\<^sub>o\<^sub>n8_def X\<^sub>P\<^sub>e\<^sub>r\<^sub>s\<^sub>o\<^sub>n9_def
-                 person1_def person2_def person3_def person4_def person5_def person6_def person7_def person8_def person9_def
-                 image_def)
  apply(simp add: including_rep_set mtSet_rep_set null_option_def bot_option_def)
  apply(simp add: oid_of_option_def oid_of_type\<^sub>O\<^sub>c\<^sub>l\<^sub>A\<^sub>n\<^sub>y_def, clarsimp)
  apply(simp add: \<sigma>\<^sub>1_def \<sigma>\<^sub>1'_def
@@ -1115,56 +1095,6 @@ proof -
                    OclAsType\<^sub>O\<^sub>c\<^sub>l\<^sub>A\<^sub>n\<^sub>y_Person)
   apply(subst cp_OclIsModifiedOnly, subst cp_OclExcluding,
     subst (asm) cp_OclIsModifiedOnly, simp add: including4 excluding1)
-
-  apply(simp add: OclValid_def defined_def
-                  X\<^sub>P\<^sub>e\<^sub>r\<^sub>s\<^sub>o\<^sub>n9_def person9_def OclSelf_at_pre_def
-                  oid0_def oid1_def oid2_def oid3_def oid4_def oid5_def oid6_def oid7_def oid8_def
-                  oid_of_option_def oid_of_type\<^sub>O\<^sub>c\<^sub>l\<^sub>A\<^sub>n\<^sub>y_def
-                  \<sigma>\<^sub>1_def OclAsType\<^sub>O\<^sub>c\<^sub>l\<^sub>A\<^sub>n\<^sub>y_\<AA>_def bot_fun_def null_fun_def bot_option_def null_option_def)
-  apply(simp only: X\<^sub>P\<^sub>e\<^sub>r\<^sub>s\<^sub>o\<^sub>n1_def X\<^sub>P\<^sub>e\<^sub>r\<^sub>s\<^sub>o\<^sub>n2_def X\<^sub>P\<^sub>e\<^sub>r\<^sub>s\<^sub>o\<^sub>n3_def X\<^sub>P\<^sub>e\<^sub>r\<^sub>s\<^sub>o\<^sub>n4_def X\<^sub>P\<^sub>e\<^sub>r\<^sub>s\<^sub>o\<^sub>n5_def X\<^sub>P\<^sub>e\<^sub>r\<^sub>s\<^sub>o\<^sub>n6_def X\<^sub>P\<^sub>e\<^sub>r\<^sub>s\<^sub>o\<^sub>n7_def X\<^sub>P\<^sub>e\<^sub>r\<^sub>s\<^sub>o\<^sub>n8_def X\<^sub>P\<^sub>e\<^sub>r\<^sub>s\<^sub>o\<^sub>n9_def
-                   person1_def person2_def person3_def person4_def person5_def person6_def person7_def person8_def person9_def)
-  apply(simp add: including_rep_set mtSet_rep_set
-                  oid0_def oid1_def oid2_def oid3_def oid4_def oid5_def oid6_def oid7_def oid8_def
-                  oid_of_option_def oid_of_type\<^sub>O\<^sub>c\<^sub>l\<^sub>A\<^sub>n\<^sub>y_def)
- done
-qed
-
-lemma "(\<sigma>\<^sub>1,\<sigma>\<^sub>1') \<Turnstile> (((X\<^sub>P\<^sub>e\<^sub>r\<^sub>s\<^sub>o\<^sub>n9 .oclAsType(OclAny)) @pre (\<lambda>x. \<lfloor>OclAsType\<^sub>O\<^sub>c\<^sub>l\<^sub>A\<^sub>n\<^sub>y_\<AA> x\<rfloor>)) \<triangleq>
-                   ((X\<^sub>P\<^sub>e\<^sub>r\<^sub>s\<^sub>o\<^sub>n9 .oclAsType(OclAny)) @post (\<lambda>x. \<lfloor>OclAsType\<^sub>O\<^sub>c\<^sub>l\<^sub>A\<^sub>n\<^sub>y_\<AA> x\<rfloor>)))"
-proof -
-
- have including4 : "\<And>a b c d \<tau>.
-        Set{\<lambda>\<tau>. \<lfloor>\<lfloor>a\<rfloor>\<rfloor>, \<lambda>\<tau>. \<lfloor>\<lfloor>b\<rfloor>\<rfloor>, \<lambda>\<tau>. \<lfloor>\<lfloor>c\<rfloor>\<rfloor>, \<lambda>\<tau>. \<lfloor>\<lfloor>d\<rfloor>\<rfloor>} \<tau> = Abs_Set_0 \<lfloor>\<lfloor> {\<lfloor>\<lfloor>a\<rfloor>\<rfloor>, \<lfloor>\<lfloor>b\<rfloor>\<rfloor>, \<lfloor>\<lfloor>c\<rfloor>\<rfloor>, \<lfloor>\<lfloor>d\<rfloor>\<rfloor>} \<rfloor>\<rfloor>"
-  apply(subst abs_rep_simp'[symmetric], simp)
- by(simp add: including_rep_set mtSet_rep_set)
-
- have excluding1: "\<And>S a b c d e \<tau>. (\<lambda>_. Abs_Set_0 \<lfloor>\<lfloor> {\<lfloor>\<lfloor>a\<rfloor>\<rfloor>, \<lfloor>\<lfloor>b\<rfloor>\<rfloor>, \<lfloor>\<lfloor>c\<rfloor>\<rfloor>, \<lfloor>\<lfloor>d\<rfloor>\<rfloor>} \<rfloor>\<rfloor>)->excluding(\<lambda>\<tau>. \<lfloor>\<lfloor>e\<rfloor>\<rfloor>) \<tau> = Abs_Set_0 \<lfloor>\<lfloor> {\<lfloor>\<lfloor>a\<rfloor>\<rfloor>, \<lfloor>\<lfloor>b\<rfloor>\<rfloor>, \<lfloor>\<lfloor>c\<rfloor>\<rfloor>, \<lfloor>\<lfloor>d\<rfloor>\<rfloor>} - {\<lfloor>\<lfloor>e\<rfloor>\<rfloor>} \<rfloor>\<rfloor>"
-  apply(simp add: OclExcluding_def)
-  apply(simp add: defined_def OclValid_def bot_fun_def bot_Set_0_def null_fun_def  null_Set_0_def false_def true_def)
-  apply(rule conjI)
-  apply(rule impI, subst (asm) Abs_Set_0_inject) apply( simp add: bot_option_def)+
-  apply(rule conjI)
-  apply(rule impI, subst (asm) Abs_Set_0_inject) apply( simp add: bot_option_def null_option_def)+
-  apply(subst Abs_Set_0_inverse, simp add: bot_option_def, simp)
- done
-
- show ?thesis
-  apply(rule framing2[where X = "Set{ X\<^sub>P\<^sub>e\<^sub>r\<^sub>s\<^sub>o\<^sub>n1 .oclAsType(OclAny)
-                       , X\<^sub>P\<^sub>e\<^sub>r\<^sub>s\<^sub>o\<^sub>n2 .oclAsType(OclAny)
-                     (*, X\<^sub>P\<^sub>e\<^sub>r\<^sub>s\<^sub>o\<^sub>n3 .oclAsType(OclAny)*)
-                       , X\<^sub>P\<^sub>e\<^sub>r\<^sub>s\<^sub>o\<^sub>n4 .oclAsType(OclAny)
-                     (*, X\<^sub>P\<^sub>e\<^sub>r\<^sub>s\<^sub>o\<^sub>n5 .oclAsType(OclAny)*)
-                       , X\<^sub>P\<^sub>e\<^sub>r\<^sub>s\<^sub>o\<^sub>n6 .oclAsType(OclAny)
-                     (*, X\<^sub>P\<^sub>e\<^sub>r\<^sub>s\<^sub>o\<^sub>n7 .oclAsType(OclAny)*)
-                     (*, X\<^sub>P\<^sub>e\<^sub>r\<^sub>s\<^sub>o\<^sub>n8 .oclAsType(OclAny)*)
-                     (*, X\<^sub>P\<^sub>e\<^sub>r\<^sub>s\<^sub>o\<^sub>n9 .oclAsType(OclAny)*)}"])
-  apply(cut_tac \<sigma>_modifiedonly2)
-  apply(simp only: OclValid_def
-                  X\<^sub>P\<^sub>e\<^sub>r\<^sub>s\<^sub>o\<^sub>n1_def X\<^sub>P\<^sub>e\<^sub>r\<^sub>s\<^sub>o\<^sub>n2_def X\<^sub>P\<^sub>e\<^sub>r\<^sub>s\<^sub>o\<^sub>n3_def X\<^sub>P\<^sub>e\<^sub>r\<^sub>s\<^sub>o\<^sub>n4_def X\<^sub>P\<^sub>e\<^sub>r\<^sub>s\<^sub>o\<^sub>n5_def X\<^sub>P\<^sub>e\<^sub>r\<^sub>s\<^sub>o\<^sub>n6_def X\<^sub>P\<^sub>e\<^sub>r\<^sub>s\<^sub>o\<^sub>n7_def X\<^sub>P\<^sub>e\<^sub>r\<^sub>s\<^sub>o\<^sub>n8_def X\<^sub>P\<^sub>e\<^sub>r\<^sub>s\<^sub>o\<^sub>n9_def
-                   person1_def person2_def person3_def person4_def person5_def person6_def person7_def person8_def person9_def
-                   OclAsType\<^sub>O\<^sub>c\<^sub>l\<^sub>A\<^sub>n\<^sub>y_Person)
-  apply(subst cp_OclIsModifiedOnly2, subst cp_OclExcluding,
-    subst (asm) cp_OclIsModifiedOnly2, simp add: including4 excluding1)
 
   apply(simp add: OclValid_def defined_def
                   X\<^sub>P\<^sub>e\<^sub>r\<^sub>s\<^sub>o\<^sub>n9_def person9_def OclSelf_at_pre_def
